create, delete, append, expunge rdy

CRDT/ORSet3.thy
@@ -80,12 +80,20 @@ lemma (in orset) append_append_commute:
   	
 lemma (in orset) append_expunge_commute:
   assumes "i1 \<noteq> mo"
-  shows "(\<langle>Append i1 e1\<rangle> \<rhd> \<langle>Expunge e2 mo i2\<rangle>) x = (\<langle>Expunge e2 mo i2\<rangle> \<rhd> \<langle>Append i1 e1\<rangle>) x"
-  using assms by(auto simp add: interpret_op_def kleisli_def op_elem_def)
+  shows "(\<langle>Append i1 e1\<rangle> \<rhd> \<langle>Expunge e2 mo i2\<rangle>) = (\<langle>Expunge e2 mo i2\<rangle> \<rhd> \<langle>Append i1 e1\<rangle>)"
+proof
+	fix x
+	show "(\<langle>Append i1 e1\<rangle> \<rhd> \<langle>Expunge e2 mo i2\<rangle>) x = (\<langle>Expunge e2 mo i2\<rangle> \<rhd> \<langle>Append i1 e1\<rangle>) x"
+		using assms by(auto simp add: interpret_op_def kleisli_def op_elem_def)
+qed
+
   	
 lemma (in orset) expunge_expunge_commute:
-  shows "(\<langle>Expunge e1 mo1 i1\<rangle> \<rhd> \<langle>Expunge e2 mo2 i2\<rangle>) x = (\<langle>Expunge e2 mo2 i2\<rangle> \<rhd> \<langle>Expunge e1 mo1 i1\<rangle>) x"
-  by(auto simp add: interpret_op_def kleisli_def op_elem_def)
+  shows "(\<langle>Expunge e1 mo1 i1\<rangle> \<rhd> \<langle>Expunge e2 mo2 i2\<rangle>) = (\<langle>Expunge e2 mo2 i2\<rangle> \<rhd> \<langle>Expunge e1 mo1 i1\<rangle>)"
+proof
+	fix x
+	show "(\<langle>Expunge e1 mo1 i1\<rangle> \<rhd> \<langle>Expunge e2 mo2 i2\<rangle>) x = (\<langle>Expunge e2 mo2 i2\<rangle> \<rhd> \<langle>Expunge e1 mo1 i1\<rangle>) x"
+  by(auto simp add: interpret_op_def kleisli_def op_elem_def) qed
 
 lemma (in orset) apply_operations_never_fails:
   assumes "xs prefix of i"
@@ -138,9 +146,47 @@ qed
 definition (in orset) added_ids :: "('id \<times> ('id, 'b) operation) event list \<Rightarrow> 'b \<Rightarrow> 'id list" where
   "added_ids es p \<equiv> List.map_filter (\<lambda>x. case x of 
 		Deliver (i, Add j e) \<Rightarrow> if e = p then Some j else None | 
-		Deliver (i, Append j e) \<Rightarrow> if e = p then Some j else None |
     Deliver (i, Expunge e mo j) \<Rightarrow> if e = p then Some j else None |
 		_ \<Rightarrow> None) es"
+	
+definition (in orset) added_files :: "('id \<times> ('id, 'b) operation) event list \<Rightarrow> 'b \<Rightarrow> 'id list" where
+    "added_files es p \<equiv> List.map_filter (\<lambda>x. case x of 
+		Deliver (i, Append j e) \<Rightarrow> if e = p then Some j else None |
+		_ \<Rightarrow> None) es"
+		
+-- {* added files simplifier *}
+  
+lemma (in orset) [simp]:
+  shows "added_files [] e = []"
+  by (auto simp: added_files_def map_filter_def)
+  	
+lemma (in orset) [simp]:
+  shows "added_files (xs @ ys) e = added_files xs e @ added_files ys e"
+    by (auto simp: added_files_def map_filter_append)
+
+lemma (in orset) added_files_Broadcast_collapse [simp]:
+  shows "added_files ([Broadcast e]) e' = []"
+  by (auto simp: added_files_def map_filter_append map_filter_def)
+    
+lemma (in orset) added_files_Deliver_Rem_collapse [simp]:
+  shows "added_files ([Deliver (i, Rem is e)]) e' = []"
+  by (auto simp: added_files_def map_filter_append map_filter_def)
+    
+lemma (in orset) added_files_Deliver_Add_collapse [simp]:
+  shows "added_files ([Deliver (i, Add j e)]) e' = []"
+  by (auto simp: added_files_def map_filter_append map_filter_def)
+
+lemma (in orset) added_files_Deliver_Expunge_collapse [simp]:
+  shows "added_files ([Deliver (i, Expunge e mo j)]) e' = []"
+  by (auto simp: added_files_def map_filter_append map_filter_def)
+    
+lemma (in orset) added_files_Deliver_Append_diff_collapse [simp]:
+  shows "e \<noteq> e' \<Longrightarrow> added_files ([Deliver (i, Append j e)]) e' = []"
+  by (auto simp: added_files_def map_filter_append map_filter_def)
+    
+lemma (in orset) added_files_Deliver_Append_same_collapse [simp]:
+  shows "added_files ([Deliver (i, Append j e)]) e = [j]"
+  by (auto simp: added_files_def map_filter_append map_filter_def)
  
 -- {* added ids simplifier *}
   
@@ -148,7 +194,7 @@ lemma (in orset) [simp]:
   shows "added_ids [] e = []"
   by (auto simp: added_ids_def map_filter_def)
   	
-lemma (in orset) [simp]:
+lemma (in orset) split_ids [simp]:
   shows "added_ids (xs @ ys) e = added_ids xs e @ added_ids ys e"
     by (auto simp: added_ids_def map_filter_append)
 
@@ -160,12 +206,12 @@ lemma (in orset) added_ids_Deliver_Rem_collapse [simp]:
   shows "added_ids ([Deliver (i, Rem is e)]) e' = []"
   by (auto simp: added_ids_def map_filter_append map_filter_def)
     
+lemma (in orset) added_ids_Deliver_Append_collapse [simp]:
+  shows "added_ids ([Deliver (i, Append j e)]) e' = []"
+  by (auto simp: added_ids_def map_filter_append map_filter_def)
+    
 lemma (in orset) added_ids_Deliver_Add_diff_collapse [simp]:
   shows "e \<noteq> e' \<Longrightarrow> added_ids ([Deliver (i, Add j e)]) e' = []"
-  by (auto simp: added_ids_def map_filter_append map_filter_def)
-  	
-lemma (in orset) added_ids_Deliver_Append_diff_collapse [simp]:
-  shows "e \<noteq> e' \<Longrightarrow> added_ids ([Deliver (i, Append j e)]) e' = []"
   by (auto simp: added_ids_def map_filter_append map_filter_def)
   	
 lemma (in orset) added_ids_Deliver_Expunge_diff_collapse [simp]:
@@ -174,10 +220,6 @@ lemma (in orset) added_ids_Deliver_Expunge_diff_collapse [simp]:
     
 lemma (in orset) added_ids_Deliver_Add_same_collapse [simp]:
   shows "added_ids ([Deliver (i, Add j e)]) e = [j]"
-  by (auto simp: added_ids_def map_filter_append map_filter_def)
-  	
-lemma (in orset) added_ids_Deliver_Append_same_collapse [simp]:
-  shows "added_ids ([Deliver (i, Append j e)]) e = [j]"
   by (auto simp: added_ids_def map_filter_append map_filter_def)
   	
 lemma (in orset) added_ids_Deliver_Expunge_same_collapse [simp]:
@@ -204,7 +246,7 @@ lemma (in orset) expunge_id_not_in_set:
 lemma (in orset) apply_operations_added_ids:
   assumes "es prefix of j"
     and "apply_operations es = Some f"
-  shows "fst (f x) \<union> snd (f x) \<subseteq> set (added_ids es x)"
+  shows "fst (f x) \<subseteq> set (added_ids es x)"
 using assms proof (induct es arbitrary: f rule: rev_induct, force)
   case (snoc x xs) thus ?case
   proof (cases x, force)
@@ -215,19 +257,59 @@ using assms proof (induct es arbitrary: f rule: rev_induct, force)
                     force split: if_split_asm simp add: op_elem_def interpret_op_def)
   qed
 qed
-	
-lemma (in orset) single_expunge:
-  assumes "xs prefix of j"
-    and "i \<in> set (added_ids xs e)"
-    and "Deliver (i, Expunge e mo i) \<in> set xs"
-    and "Deliver (i, Expunge e mo2 i) \<in> set xs"
-  shows "mo = mo2"
-  	sorry
+  
+lemma (in orset) apply_operations_added_files:
+  assumes "es prefix of j"
+    and "apply_operations es = Some f"
+  shows "snd (f x) \<subseteq> set (added_files es x)"
+using assms proof (induct es arbitrary: f rule: rev_induct, force)
+  case (snoc x xs) thus ?case
+  proof (cases x, force)
+    case (Deliver e)
+    moreover obtain a b where "e = (a, b)" by force
+    ultimately show ?thesis
+      using snoc by(case_tac b; clarsimp simp: interp_msg_def split: bind_splits,
+                    force split: if_split_asm simp add: op_elem_def interpret_op_def)
+  qed
+qed
 
+lemma (in orset) Deliver_added_files:
+  assumes "xs prefix of j"
+    and "i \<in> set (added_files xs e)"
+  shows "Deliver (i, Append i e) \<in> set xs"
+using assms proof (induct xs rule: rev_induct, clarsimp)
+  case (snoc x xs) thus ?case
+  proof (cases x, force)
+    case X: (Deliver e')
+    moreover obtain a b where E: "e' = (a, b)" by force
+    ultimately show ?thesis
+      using snoc apply (case_tac b; clarify)
+       apply (simp,metis prefix_of_appendD)
+        apply force using  append_id_valid
+        apply simp using E 
+      apply (metis added_files_Deliver_Append_diff_collapse added_files_Deliver_Append_same_collapse empty_iff in_set_conv_decomp list.set(1) prefix_of_appendD set_ConsD)
+      	apply simp using E apply_operations_added_files
+      by blast
+  qed
+qed
+  
+
+lemma (in orset) Broadcast_Expunge_Deliver_prefix_closed:
+  assumes "xs @ [Broadcast (i, Expunge e mo i)] prefix of j"
+  shows "Deliver (mo, Append mo e) \<in> set xs"
+proof -  
+  obtain y where "apply_operations xs = Some y"
+    using assms broadcast_only_valid_msgs by blast
+  moreover hence "mo \<in> snd (y e)"
+    using broadcast_only_valid_msgs[of xs "(i, Expunge e mo i)" j] valid_behaviours_def[of y "(i, Expunge e mo i)"] using assms by auto
+  ultimately show ?thesis
+    using assms Deliver_added_files apply_operations_added_files by blast
+qed
+            
 lemma (in orset) Deliver_added_ids:
   assumes "xs prefix of j"
     and "i \<in> set (added_ids xs e)"
-  shows "Deliver (i, Add i e) \<in> set xs \<or> Deliver (i, Append i e) \<in> set xs \<or> Deliver (i, Expunge e mo i) \<in> set xs"
+  shows "Deliver (i, Add i e) \<in> set xs \<or> (\<exists> mo . Deliver (i, Expunge e mo i) \<in> set xs)"
 using assms proof (induct xs rule: rev_induct, clarsimp)
   case (snoc x xs) thus ?case
   proof (cases x, force)
@@ -237,35 +319,19 @@ using assms proof (induct xs rule: rev_induct, clarsimp)
       using snoc apply (case_tac b; clarify)
        apply (simp,metis added_ids_Deliver_Add_diff_collapse added_ids_Deliver_Add_same_collapse
               empty_iff list.set(1) set_ConsD add_id_valid in_set_conv_decomp prefix_of_appendD)
-       apply force using added_ids_Deliver_Append_diff_collapse added_ids_Deliver_Append_same_collapse append_id_valid
+       apply force using  append_id_valid 
       	
-       apply (simp, metis (no_types, lifting) Diff_eq_empty_iff Diff_iff Un_iff list.set(1) list.set_intros(1) prefix_of_appendD set_ConsD set_append subset_Compl_singleton)
-
-    proof (clarsimp)
-    	fix x41 x42 x43
-    		assume A1: "i \<in> set (added_ids xs e) \<or> i \<in> set (added_ids [Deliver (a, Expunge x41 x42 x43)] e)"
-       "(xs prefix of j \<Longrightarrow> i \<in> set (added_ids xs e) \<Longrightarrow> Deliver (i, Append i e) \<in> set xs)"
-       "xs @ [Deliver (a, Expunge x41 x42 x43)] prefix of j"
-       "x = Deliver (a, Expunge x41 x42 x43)"
-       "e' = (a, Expunge x41 x42 x43)"
-       "b = Expunge x41 x42 x43"
-       "Deliver (i, Add i e) \<notin> set xs" "(mo = x42 \<longrightarrow> e = x41 \<longrightarrow> i = a \<longrightarrow> a \<noteq> x43)" "Deliver (i, Expunge e mo i) \<notin> set xs "       
-       
-       hence "i \<in> set (added_ids xs e)" using snoc apply (case_tac "mo = x42") 
-       		apply (metis Un_iff added_ids_Deliver_Expunge_diff_collapse added_ids_Deliver_Expunge_same_collapse empty_iff expunge_id_valid list.set(1) list.set_intros(1) set_ConsD set_append)
-       		 apply (case_tac "e \<noteq> x41") 
-       	 apply simp apply (case_tac "i \<noteq> a") apply simp
-       	 apply (metis Un_iff expunge_id_valid list.set_intros(1) set_append) apply (case_tac "a \<noteq> x43") apply simp using expunge_id_not_in_set using single_expunge
-      	thus "Deliver (i, Append i e) \<in> set xs" using snoc
-      		using A1(2) by blast
-      qed
+       apply (simp, metis (no_types, lifting)  prefix_of_appendD)
+      
+      apply (simp)
+      by (metis Un_iff added_ids_Deliver_Expunge_diff_collapse added_ids_Deliver_Expunge_same_collapse empty_iff expunge_id_valid list.set(1) list.set_intros(1) prefix_of_appendD set_ConsD set_append)
   qed
 qed
 
 lemma (in orset) Broadcast_Deliver_prefix_closed:
   assumes "xs @ [Broadcast (r, Rem ix e)] prefix of j"
     and "i \<in> ix"
-  shows "Deliver (i, Add i e) \<in> set xs \<or> Deliver (i, Append i e) \<in> set xs"
+  shows "Deliver (i, Add i e) \<in> set xs \<or> Deliver (i, Append i e) \<in> set xs \<or> (\<exists> mo . Deliver (i, Expunge e mo i) \<in> set xs)"
 proof -  
   obtain y where "apply_operations xs = Some y"
     using assms broadcast_only_valid_msgs by blast
@@ -273,23 +339,27 @@ proof -
     by (metis (mono_tags, lifting) assms(1) broadcast_only_valid_msgs operation.case(2) option.simps(1)
      valid_behaviours_def case_prodD)
   ultimately show ?thesis
-    using assms Deliver_added_ids apply_operations_added_ids by blast
+    using assms Deliver_added_ids apply_operations_added_ids
+    by (metis Deliver_added_files Un_iff apply_operations_added_files le_iff_sup prefix_of_appendD)
 qed
 	
+(*
 lemma (in orset) Broadcast_Deliver_prefix_closed2:
   assumes "xs prefix of j"
     and "Broadcast (r, Rem ix e) \<in> set xs"
     and "i \<in> ix"
-  shows "Deliver (i, Add i e) \<in> set xs \<or> Deliver (i, Append i e) \<in> set xs"
+  shows "Deliver (i, Add i e) \<in> set xs \<or> Deliver (i, Append i e) \<in> set xs \<or> (\<exists> mo .Deliver (i, Expunge e mo i) \<in> set xs)"
 using assms Broadcast_Deliver_prefix_closed by (induction xs rule: rev_induct; force)
-
+*)
+  
 lemma (in orset) ids_are_unique:
     assumes "xs prefix of j"
     and "(i, Add i e1) \<in> set (node_deliver_messages xs)" 
     and "(l, Append l e2) \<in> set (node_deliver_messages xs)"
-  shows "i \<noteq> l"
-  	using assms delivery_has_a_cause events_before_exist prefix_msg_in_history
-  	by (metis fst_conv msg_id_unique  operation.distinct(3) prod.inject)
+    and "(k, Expunge e3 mo k) \<in> set (node_deliver_messages xs)"
+  shows "i \<noteq> l \<and> i \<noteq> k \<and> l \<noteq> k"
+  	using assms delivery_has_a_cause events_before_exist prefix_msg_in_history 
+  	by (metis (no_types, lifting) fst_conv network.msg_id_unique network_axioms operation.distinct(11) operation.distinct(3) operation.distinct(5) prod.inject)
 	
 lemma (in orset) concurrent_add_remove_independent_technical:
   assumes "i \<in> is"
@@ -299,7 +369,7 @@ lemma (in orset) concurrent_add_remove_independent_technical:
 proof -
   obtain pre k where "pre@[Broadcast (ir, Rem is e)] prefix of k"
     using assms delivery_has_a_cause events_before_exist prefix_msg_in_history by blast
-  moreover hence "Deliver (i, Add i e) \<in> set pre \<or> Deliver (i, Append i e) \<in> set pre"
+  moreover hence "Deliver (i, Add i e) \<in> set pre \<or> Deliver (i, Append i e) \<in> set pre \<or> (\<exists> mo . Deliver (i, Expunge e mo i) \<in> set pre)"
     using Broadcast_Deliver_prefix_closed assms(1) by auto    	
   hence "Deliver (i, Add i e) \<in> set pre" using assms(2) assms(3) ids_are_unique
   	by (smt calculation fst_conv network.delivery_has_a_cause network.msg_id_unique network_axioms prefix_elem_to_carriers prefix_msg_in_history prefix_of_appendD)
@@ -315,13 +385,69 @@ lemma (in orset) concurrent_append_remove_independent_technical:
 proof -
   obtain pre k where "pre@[Broadcast (ir, Rem is e)] prefix of k"
     using assms delivery_has_a_cause events_before_exist prefix_msg_in_history by blast
-  moreover hence "Deliver (i, Add i e) \<in> set pre \<or> Deliver (i, Append i e) \<in> set pre "
+  moreover hence "Deliver (i, Add i e) \<in> set pre \<or> Deliver (i, Append i e) \<in> set pre \<or> (\<exists> mo . Deliver (i, Expunge e mo i) \<in> set pre)"
     using Broadcast_Deliver_prefix_closed assms(1) by auto
     	
   hence "Deliver (i, Append i e) \<in> set pre" using assms(2) assms(3) ids_are_unique
   	by (smt calculation fst_conv network.delivery_has_a_cause network.msg_id_unique network_axioms prefix_elem_to_carriers prefix_msg_in_history prefix_of_appendD)
   ultimately show ?thesis
     using hb.intros(2) events_in_local_order by blast
+qed
+	
+lemma (in orset) concurrent_append_expunge_independent_technical:
+  assumes "i = mo"
+    and "xs prefix of j"
+    and "(i, Append i e) \<in> set (node_deliver_messages xs)" and "(r, Expunge e mo r) \<in> set (node_deliver_messages xs)"
+  shows "hb (i, Append i e) (r, Expunge e mo r)"
+proof -
+  obtain pre k where "pre@[Broadcast (r, Expunge e mo r)] prefix of k"
+    using assms delivery_has_a_cause events_before_exist prefix_msg_in_history by blast
+  moreover hence "Deliver (mo, Append mo e) \<in> set pre"
+    using Broadcast_Expunge_Deliver_prefix_closed assms(1) by auto
+    	
+  hence "Deliver (i, Append i e) \<in> set pre" using assms(2) assms(3) ids_are_unique
+  	using assms(1) by blast
+  ultimately show ?thesis
+    using hb.intros(2) events_in_local_order by blast
+qed
+  
+lemma (in orset) concurrent_expunge_remove_independent_technical:
+  assumes "i \<in> is"
+    and "xs prefix of j"
+    and "(i, Expunge e mo i) \<in> set (node_deliver_messages xs)" and "(ir, Rem is e) \<in> set (node_deliver_messages xs)"
+  shows "hb (i, Expunge e mo i) (ir, Rem is e)"
+proof -
+  obtain pre k where "pre@[Broadcast (ir, Rem is e)] prefix of k"
+    using assms delivery_has_a_cause events_before_exist prefix_msg_in_history by blast
+  moreover hence "Deliver (i, Add i e) \<in> set pre \<or> Deliver (i, Append i e) \<in> set pre \<or> (\<exists> mo . Deliver (i, Expunge e mo i) \<in> set pre)"
+    using Broadcast_Deliver_prefix_closed assms(1) by auto
+    	
+  hence "Deliver (i, Expunge e mo i) \<in> set pre" using assms(2) assms(3) ids_are_unique
+  	by (smt calculation fst_conv network.delivery_has_a_cause network.msg_id_unique network_axioms prefix_elem_to_carriers prefix_msg_in_history prefix_of_appendD)
+  ultimately show ?thesis
+    using hb.intros(2) events_in_local_order by blast
+qed
+  
+lemma (in orset) expunge_rem_ids_imply_messages_same:
+  assumes "i \<in> is"
+    and "xs prefix of j"
+    and "(i, Expunge e1 mo i) \<in> set (node_deliver_messages xs)" and "(ir, Rem is e2) \<in> set (node_deliver_messages xs)"
+  shows "e1 = e2"
+proof -
+  obtain pre k where "pre@[Broadcast (ir, Rem is e2)] prefix of k"
+    using assms delivery_has_a_cause events_before_exist prefix_msg_in_history by blast
+  
+   moreover hence "Deliver (i, Add i e2) \<in> set pre \<or> Deliver (i, Append i e2) \<in> set pre \<or> (\<exists> mo . Deliver (i, Expunge e2 mo i) \<in> set pre)"
+    using Broadcast_Deliver_prefix_closed assms(1)
+    by (meson orset.Broadcast_Deliver_prefix_closed orset_axioms)
+    	
+  hence "Deliver (i, Expunge e2 mo i) \<in> set pre" using assms(2) assms(3) assms(1) ids_are_unique 
+    by (smt calculation delivery_has_a_cause fst_conv network.msg_id_unique network_axioms operation.distinct(11) operation.distinct(5) operation.inject(4) prefix_elem_to_carriers prefix_msg_in_history prefix_of_appendD prod.inject)
+
+  	moreover have "Deliver(i, Expunge e1 mo i) \<in> set (history j)"
+    using assms(2) assms(3) prefix_msg_in_history by blast
+  ultimately show ?thesis
+    by (metis (no_types, lifting) delivery_has_a_cause fst_conv network.msg_id_unique network_axioms operation.inject(4) prefix_elem_to_carriers prefix_of_appendD prod.inject)
 qed
 	
 (*
@@ -345,7 +471,7 @@ lemma (in orset) add_rem_ids_imply_messages_same:
 proof -
   obtain pre k where "pre@[Broadcast (ir, Rem is e2)] prefix of k"
     using assms delivery_has_a_cause events_before_exist prefix_msg_in_history by blast
-  moreover hence "Deliver (i, Add i e2) \<in> set pre \<or> Deliver (i, Append i e2) \<in> set pre"
+  moreover hence "Deliver (i, Add i e2) \<in> set pre \<or> Deliver (i, Append i e2) \<in> set pre \<or> (\<exists> mo . Deliver (i, Expunge e2 mo i) \<in> set pre)"
     using Broadcast_Deliver_prefix_closed assms(1) ids_are_unique by blast
   hence "Deliver (i, Add i e2) \<in> set pre" using assms(1) assms(2) assms(3) ids_are_unique
   	by (smt calculation fst_conv network.delivery_has_a_cause network.msg_id_unique network_axioms operation.simps(10) operation.simps(8) prefix_elem_to_carriers prefix_msg_in_history prefix_of_appendD prod.simps(1))
@@ -365,19 +491,43 @@ proof -
   obtain pre k where "pre@[Broadcast (ir, Rem is e2)] prefix of k"
     using assms delivery_has_a_cause events_before_exist prefix_msg_in_history by blast
   
-   moreover hence "Deliver (i, Add i e2) \<in> set pre \<or> Deliver (i, Append i e2) \<in> set pre"
+   moreover hence "Deliver (i, Add i e2) \<in> set pre \<or> Deliver (i, Append i e2) \<in> set pre \<or> (\<exists> mo . Deliver (i, Expunge e2 mo i) \<in> set pre)"
     using Broadcast_Deliver_prefix_closed assms(1)
     by (meson orset.Broadcast_Deliver_prefix_closed orset_axioms)
     	
   hence "Deliver (i, Append i e2) \<in> set pre" using assms(2) assms(3) assms(1) ids_are_unique
-  by (smt calculation fst_conv network.delivery_has_a_cause network.msg_id_unique network_axioms operation.simps(8) prefix_elem_to_carriers prefix_msg_in_history prefix_of_appendD prod.simps(1))
-
+  	by (smt calculation fst_conv network.delivery_has_a_cause network.msg_id_unique network_axioms operation.distinct(11) operation.distinct(3) prefix_elem_to_carriers prefix_msg_in_history prefix_of_appendD prod.inject)
+      
+      
   	moreover have "Deliver (i, Append i e1) \<in> set (history j)"
     using assms(2) assms(3) prefix_msg_in_history by blast
   ultimately show ?thesis
     by (metis (no_types, lifting) fst_conv network.delivery_has_a_cause network.msg_id_unique network_axioms operation.inject(3) prefix_elem_to_carriers prefix_of_appendD prod.inject)
 qed
 
+lemma (in orset) append_expunge_ids_imply_messages_same:
+  assumes "i = mo"
+    and "xs prefix of j"
+    and "(i, Append i e1) \<in> set (node_deliver_messages xs)" and "(r, Expunge e2 mo r) \<in> set (node_deliver_messages xs)"
+  shows "e1 = e2"
+proof -
+  obtain pre k where "pre@[Broadcast (r, Expunge e2 mo r)] prefix of k"
+    using assms delivery_has_a_cause events_before_exist prefix_msg_in_history by blast
+  
+   moreover hence "Deliver (mo, Append mo e2) \<in> set pre"
+    using Broadcast_Expunge_Deliver_prefix_closed assms(1)
+    by (meson orset.Broadcast_Deliver_prefix_closed orset_axioms)
+    	
+  hence "Deliver (i, Append i e2) \<in> set pre" using assms(2) assms(3) assms(1) ids_are_unique
+  	by blast
+      
+      
+  	moreover have "Deliver (i, Append i e1) \<in> set (history j)"
+    using assms(2) assms(3) prefix_msg_in_history by blast
+  ultimately show ?thesis
+    by (metis (no_types, lifting) fst_conv network.delivery_has_a_cause network.msg_id_unique network_axioms operation.inject(3) prefix_elem_to_carriers prefix_of_appendD prod.inject)
+qed
+	
 corollary (in orset) concurrent_add_remove_independent:
   assumes "\<not> hb (i, Add i e1) (ir, Rem is e2)" and "\<not> hb (ir, Rem is e2) (i, Add i e1)"
     and "xs prefix of j"
@@ -386,11 +536,25 @@ corollary (in orset) concurrent_add_remove_independent:
   using assms add_rem_ids_imply_messages_same concurrent_add_remove_independent_technical by fastforce
   	
 corollary (in orset) concurrent_append_remove_independent:
-  assumes "\<not> hb (i, Append i e1) (ir, Rem is e2)" and "\<not> hb (ir, Rem is e2) (i, Add i e1)"
+  assumes "\<not> hb (i, Append i e1) (ir, Rem is e2)" and "\<not> hb (ir, Rem is e2) (i, Append i e1)"
     and "xs prefix of j"
     and "(i, Append i e1) \<in> set (node_deliver_messages xs)" and "(ir, Rem is e2) \<in> set (node_deliver_messages xs)"
   shows "i \<notin> is"
   using assms append_rem_ids_imply_messages_same concurrent_append_remove_independent_technical by fastforce
+  	
+corollary (in orset) concurrent_append_expunge_independent:
+  assumes "\<not> hb (i, Append i e1) (r, Expunge e2 mo r)" and "\<not> hb (r, Expunge e2 mo r) (i, Append i e1)"
+    and "xs prefix of j"
+    and "(i, Append i e1) \<in> set (node_deliver_messages xs)" and "(r, Expunge e2 mo r) \<in> set (node_deliver_messages xs)"
+  shows "i \<noteq> mo"
+  using assms append_expunge_ids_imply_messages_same concurrent_append_expunge_independent_technical by fastforce
+    
+corollary (in orset) concurrent_expunge_remove_independent:
+  assumes "\<not> hb (i, Expunge e1 mo i) (ir, Rem is e2)" and "\<not> hb (ir, Rem is e2) (i, Expunge e1 mo i)"
+    and "xs prefix of j"
+    and "(i, Expunge e1 mo i) \<in> set (node_deliver_messages xs)" and "(ir, Rem is e2) \<in> set (node_deliver_messages xs)"
+  shows "i \<notin> is"
+  using assms expunge_rem_ids_imply_messages_same concurrent_expunge_remove_independent_technical by fastforce
 
 lemma (in orset) concurrent_operations_commute:
   assumes "xs prefix of i"
@@ -400,12 +564,20 @@ proof -
     assume "(a, b) \<in> set (node_deliver_messages xs)"
            "(x, y) \<in> set (node_deliver_messages xs)"
            "hb.concurrent (a, b) (x, y)"
-    hence "interp_msg (a, b) \<rhd> interp_msg (x, y) = interp_msg (x, y) \<rhd> interp_msg (a, b)"
+    hence "interp_msg (a, b) \<rhd> interp_msg (x, y) = interp_msg (x, y) \<rhd> interp_msg (a, b)" sledgehammer
       apply(unfold interp_msg_def, case_tac "b"; case_tac "y"; simp add: add_add_commute rem_rem_commute append_append_commute add_append_commute add_expunge_commute expunge_expunge_commute hb.concurrent_def)
        apply (metis (full_types) add_id_valid add_rem_commute assms concurrent_add_remove_independent prefix_contains_msg)+
-       apply (metis append_id_valid append_rem_ids_imply_messages_same assms concurrent_append_remove_independent_technical prefix_contains_msg rem_append_commute)
-       by (metis append_id_valid append_rem_ids_imply_messages_same assms concurrent_append_remove_independent_technical prefix_contains_msg rem_append_commute)
-      
+            apply (metis append_id_valid append_rem_ids_imply_messages_same assms concurrent_append_remove_independent_technical prefix_contains_msg rem_append_commute)
+        
+           apply (metis assms concurrent_expunge_remove_independent expunge_id_valid network.prefix_contains_msg network_axioms orset.rem_expunge_commute orset_axioms)
+        
+          apply (metis append_id_valid append_rem_ids_imply_messages_same assms concurrent_append_remove_independent_technical prefix_contains_msg rem_append_commute)
+          apply (metis append_id_valid expunge_id_valid append_expunge_ids_imply_messages_same assms concurrent_append_expunge_independent_technical prefix_contains_msg append_expunge_commute)
+        
+          
+        apply (metis assms concurrent_expunge_remove_independent expunge_id_valid prefix_contains_msg rem_expunge_commute)
+       by (metis append_expunge_commute append_id_valid assms concurrent_append_expunge_independent expunge_id_valid prefix_contains_msg)
+              
   } thus ?thesis
     by(fastforce simp: hb.concurrent_ops_commute_def)
 qed
